src/Lustre/Denot/Abs.v
@@ -291,32 +291,31 @@ Section Abs_indep_node.
 
  (* utile pour les cas récursifs *)
   Lemma lift_IH :
-    forall ins es envG envI bs env aenv,
-      Forall (fun e => denot_exp G ins e envG (APP_env abs_env envI) (cons false bs) aenv
-                    <= lift (CONS abs) (denot_exp G ins e envG envI bs env)) es ->
-      denot_exps G ins es envG (APP_env abs_env envI) (cons false bs) aenv
-      <= lift (CONS abs) (denot_exps G ins es envG envI bs env).
+    forall ins es envG envI env aenv,
+      Forall (fun e => denot_exp G ins e envG (APP_env abs_env envI) aenv
+                    <= lift (CONS abs) (denot_exp G ins e envG envI env)) es ->
+      denot_exps G ins es envG (APP_env abs_env envI) aenv
+      <= lift (CONS abs) (denot_exps G ins es envG envI env).
   Proof.
     induction es; intros * Hf; inv Hf.
-    - now rewrite 2 denot_exps_nil, map_eq_cons.
+    - now rewrite 2 denot_exps_nil.
     - rewrite 2 denot_exps_eq.
       setoid_rewrite lift_app; auto.
   Qed.
 
   (* idem *)
   Lemma lift_IHs :
-    forall ins (ess : list (enumtag * _)) n envG envI bs env aenv,
+    forall ins (ess : list (enumtag * _)) n envG envI env aenv,
       Forall (fun es =>
                 Forall (fun e =>
-                          denot_exp G ins e envG (APP_env abs_env envI) (cons false bs) aenv
-                          <= lift (CONS abs) (denot_exp G ins e envG envI bs env)) (snd es)) ess ->
-      denot_expss G ins ess n envG (APP_env abs_env envI) (cons false bs) aenv
-      <= lift (lift (CONS abs)) (denot_expss G ins ess n envG envI bs env).
+                          denot_exp G ins e envG (APP_env abs_env envI) aenv
+                          <= lift (CONS abs) (denot_exp G ins e envG envI env)) (snd es)) ess ->
+      denot_expss G ins ess n envG (APP_env abs_env envI) aenv
+      <= lift (lift (CONS abs)) (denot_expss G ins ess n envG envI env).
   Proof.
     intros * Hf.
     induction ess as [|(x,es)]; inv Hf.
-    - rewrite 2 denot_expss_nil, map_eq_cons.
-      cbn; now rewrite lift_nprod_const.
+    - rewrite 2 denot_expss_nil; auto.
     - rewrite 2 denot_expss_eq.
       unfold eq_rect.
       cases; subst.
@@ -324,8 +323,6 @@ Section Abs_indep_node.
           |-_ <= _ (_ (_ ?a) ?b) =>
             setoid_rewrite (lift_cons (lift (CONS abs)) _ a b)
         end; auto using lift_IH.
-      + simpl (length _).
-        now rewrite 2 lift_nprod_const, map_eq_cons.
   Qed.
 
   Lemma var_abs_le :
@@ -341,23 +338,23 @@ Section Abs_indep_node.
   Qed.
 
   Lemma abs_indep_exp :
-    forall Γ ins e envI bs env aenv,
+    forall Γ ins e envI env aenv,
       wt_exp G Γ e ->
       wl_exp G e ->
       aenv <= APP_env abs_env env ->
-      denot_exp G ins e envG (APP_env abs_env envI) (cons false bs) aenv
-      <= lift (CONS abs) (denot_exp G ins e envG envI bs env).
+      denot_exp G ins e envG (APP_env abs_env envI) aenv
+      <= lift (CONS abs) (denot_exp G ins e envG envI env).
   Proof.
     intros * Hwt Hwl Hle.
     induction e using exp_ind2; try apply Dbot.
     - (* Econst *)
       rewrite 2 denot_exp_eq.
       unfold sconst.
-      rewrite MAP_map, map_eq_cons; auto.
+      rewrite MAP_map, bss_app_abs, map_eq_cons; auto.
     - (* Eenum *)
       rewrite 2 denot_exp_eq.
       unfold sconst.
-      rewrite MAP_map, map_eq_cons; auto.
+      rewrite MAP_map, bss_app_abs, map_eq_cons; auto.
     - (* Evar *)
       rewrite 2 denot_exp_eq.
       now apply var_abs_le.
@@ -409,7 +406,7 @@ Section Abs_indep_node.
     - (* Emerge *)
       inv Hwt. inv Hwl.
       rewrite 2 (denot_exp_eq _ _ (Emerge _ _ _)).
-      pose proof (IH := lift_IHs ins es (length tys) envG envI bs env aenv).
+      pose proof (IH := lift_IHs ins es (length tys) envG envI env aenv).
       eassert (Le: _ <= _); [apply IH; simpl_Forall; auto|clear IH].
       cbv zeta; revert Le.
       gen_sub_exps; intros t1 t2 Le.
@@ -423,7 +420,7 @@ Section Abs_indep_node.
       apply Forall_impl_inside with (P := wt_exp _ _) in H0; auto.
       apply Forall_impl_inside with (P := wl_exp _ ) in H0; auto.
       apply lift_IH in H0.
-      pose proof (IH := lift_IHs ins es (length tys) envG envI bs env aenv).
+      pose proof (IH := lift_IHs ins es (length tys) envG envI env aenv).
       eassert (Le: _ <= _); [apply IH; simpl_Forall; auto|clear H IH].
       rewrite 2 (denot_exp_eq _ _ (Ecase _ _ _ _)).
       cbv zeta; revert IHe H0 Le; gen_sub_exps.
@@ -437,7 +434,7 @@ Section Abs_indep_node.
       { (* Ecase total *)
       inv Hwt. inv Hwl.
       rewrite 2 (denot_exp_eq _ _ (Ecase _ _ _ _)).
-      pose proof (IH := lift_IHs ins es (length tys) envG envI bs env aenv).
+      pose proof (IH := lift_IHs ins es (length tys) envG envI env aenv).
       eassert (Le: _ <= _); [apply IH; simpl_Forall; auto|clear IH].
       cbv zeta; revert IHe Le; gen_sub_exps.
       take (numstreams e = 1) and rewrite it.
@@ -465,15 +462,15 @@ Section Abs_indep_node.
   Qed.
 
   Corollary abs_indep_exps :
-    forall Γ ins es envI bs env aenv,
+    forall Γ ins es envI env aenv,
       Forall (wt_exp G Γ) es ->
       Forall (wl_exp G) es ->
       aenv <= APP_env abs_env env ->
-      denot_exps G ins es envG (APP_env abs_env envI) (cons false bs) aenv
-      <= lift (CONS abs) (denot_exps G ins es envG envI bs env).
+      denot_exps G ins es envG (APP_env abs_env envI) aenv
+      <= lift (CONS abs) (denot_exps G ins es envG envI env).
   Proof.
     induction es as [|e es]; intros * Hwt Hwl Le; inv Hwl; inv Hwt.
-    - now rewrite 2 denot_exps_nil, map_eq_cons.
+    - now rewrite 2 denot_exps_nil.
     - rewrite 2 denot_exps_eq.
       match goal with
         |-_ <= _ (_ (_ ?a) ?b) => setoid_rewrite (lift_app (CONS abs) _ a _ b)
@@ -482,13 +479,13 @@ Section Abs_indep_node.
   Qed.
 
   Lemma abs_indep_block :
-    forall Γ ins blk envI bs env aenv acc aacc,
+    forall Γ ins blk envI env aenv acc aacc,
       wt_block G Γ blk ->
       wl_block G blk ->
       aenv <= APP_env abs_env env ->
       aacc <= APP_env abs_env acc ->
-      denot_block G ins blk envG (APP_env abs_env envI) (cons false bs) aenv aacc
-      <= APP_env abs_env (denot_block G ins blk envG envI bs env acc).
+      denot_block G ins blk envG (APP_env abs_env envI) aenv aacc
+      <= APP_env abs_env (denot_block G ins blk envG envI env acc).
   Proof.
     intros * Hwt Hwl Lee Lea.
     rewrite 2 denot_block_eq; cases.
@@ -519,7 +516,6 @@ Section Abs_indep_node.
     induction l0 as [|b blks]; simpl (fold_right _ _ _).
     - apply Dbot.
     - do 2 take (Forall _ (_::_)) and inv it.
-      rewrite bss_app_abs.
       eapply abs_indep_block; eauto 2.
   Qed.
 
